Native support for bit fields (#400)
This big PR adds support for bit fields in structs and unions to
the verified part of CompCert, namely the CompCert C and Clight
languages.

The compilation of bit field accesses to normal integer accesses +
shifts and masks is done and proved correct as part of the Cshmgen
pass.

The layout of bit fields in memory is done by the functions in module
Ctypes. It follows the ELF ABI layout algorithm. As a bonus, basic
soundness properties of the layout are shown, such as "two different
bit fields do not overlap" or "a bit field and a regular field do not
overlap".

All this replaces the previous emulation of bit fields by
source-to-source rewriting in the unverified front-end of CompCert
(module cparse/Bitfield.ml). This emulation was prone to errors (see
nonstandard layout instead.

The core idea for the PR is that expressions in l-value position
denote not just a block, a byte offset and a type, but also a bitfield
designator saying whether all the bits of the type are accessed
(designator Full) or only some of its bits (designator
Bits). Designators of the Bits kind appear when the l-value is a bit
field access; the bit width and bit offset in Bits are computed by the
functions in Ctypes that implement the layout algorithm.

Consequently, both in the semantics of CompCert C and Clight and in
the SimplExpr, SimplLocals and Cshmgen compilation passes, pairs of a
type and a bitfield designator are used in a number of places where a
single type was used before.

The introduction of bit fields has a big impact on static
initialization (module cfrontend/Initializers.v), which had to be
rewritten in large part, along with its soundness proof
(cfrontend/Initializersproof.v).

Both static initialization and run-time manipulation of bit fields are
tested in test/abi using differential testing against GCC and
randomly-generated structs.

This work exposed subtle interactions between bit fields and the
volatile modifier. Currently, the volatile modifier is ignored when
accessing a bit field (and a warning is printed at compile-time), just
like it is ignored when accessing a struct or union as a r-value.

Currently, the natural alignment of bit fields and their storage units
cannot be modified with the aligned attribute. _Alignas on bit fields
is rejected as per C11, and the packed modifier cannot be applied to a
struct containing bit fields.

cfrontend/PrintCsyntax.ml
@@ -204,7 +204,7 @@ let rec expr p (prec, e) =
   then fprintf p "@[<hov 2>("
   else fprintf p "@[<hov 2>";
   begin match e with
-  | Eloc(b, ofs, _) ->
+  | Eloc(b, ofs, _, _) ->
       fprintf p "<loc%a>" !print_pointer_hook (b, ofs)
   | Evar(id, _) ->
       fprintf p "%s" (extern_atom id)
@@ -534,13 +534,18 @@ let struct_or_union = function Struct -> "struct" | Union -> "union"
 let declare_composite p (Composite(id, su, m, a)) =
   fprintf p "%s %s;@ " (struct_or_union su) (extern_atom id)
 
+let print_member p = function
+  | Member_plain(id, ty) ->
+      fprintf p "@ %s;" (name_cdecl (extern_atom id) ty)
+  | Member_bitfield(id, sz, sg, attr, w, _is_padding) ->
+      fprintf p "@ %s : %s;"
+              (name_cdecl (extern_atom id) (Tint(sz, sg, attr)))
+              (Z.to_string w)
+
 let define_composite p (Composite(id, su, m, a)) =
   fprintf p "@[<v 2>%s %s%s {"
           (struct_or_union su) (extern_atom id) (attributes a);
-  List.iter
-    (fun (fid, fty) ->
-      fprintf p "@ %s;" (name_cdecl (extern_atom fid) fty))
-    m;
+  List.iter (print_member p) m;
   fprintf p "@;<0 -2>};@]@ @ "
 
 let print_program p prog =
