test/abi/genlayout.ml
@@ -1,0 +1,158 @@
+open Printf
+
+type typ = Bool | Char | Short | Int
+
+type field =
+  | Plain of typ
+  | Bitfield of typ * int
+  | Padding of typ * int
+
+type struct_ = field list
+
+(* Concise description of a struct *)
+
+let print_typ oc = function
+  | Bool -> fprintf oc "b"
+  | Char -> fprintf oc "c"
+  | Short -> fprintf oc "s"
+  | Int -> fprintf oc "i"
+
+let print_padding_typ oc = function
+  | Bool -> fprintf oc "B"
+  | Char -> fprintf oc "C"
+  | Short -> fprintf oc "S"
+  | Int -> fprintf oc "I"
+
+let print_field oc = function
+  | Plain t -> print_typ oc t
+  | Bitfield(t, w) -> fprintf oc "%a%d" print_typ t w
+  | Padding(t, w) -> fprintf oc "%a%d" print_padding_typ t w
+
+let rec print_struct oc = function
+  | [] -> ()
+  | f :: s -> print_field oc f; print_struct oc s
+
+(* Printing a struct in C syntax *)
+
+let c_typ oc = function
+  | Bool -> fprintf oc "_Bool"
+  | Char -> fprintf oc "char"
+  | Short -> fprintf oc "short"
+  | Int -> fprintf oc "int"
+
+let c_name oc n = fprintf oc "%c" (Char.chr (Char.code 'a' + n))
+
+let c_field oc n = function
+  | Plain t ->
+      fprintf oc "  %a %a;\n" c_typ t c_name n; 
+      n + 1
+  | Bitfield(t, w) -> 
+      fprintf oc "  %a %a:%d;\n" c_typ t c_name n w;
+      n + 1
+  | Padding(t, w) ->
+      fprintf oc "  %a :%d;\n" c_typ t w;
+      n
+
+let c_struct oc s =
+  fprintf oc "struct %a {\n" print_struct s;
+  let rec c_str n = function
+    | [] -> ()
+    | f :: s -> let n' = c_field oc n f in c_str n' s in
+  c_str 0 s;
+  fprintf oc "};\n"
+
+(* Random generation of structs *)
+
+let random_1_8 () =
+  let n1 = Random.bits() in
+  let n2 = n1 lsr 2 in
+  match n1 land 3 with
+  | 0 -> 1
+  | 1 -> 2 + (n2 land 1)   (* 2-3 *)
+  | 2 -> 4 + (n2 land 1)   (* 4-5 *)
+  | 3 -> 6 + (n2 mod 3)    (* 6-8 *)
+  | _ -> assert false
+
+let random_1_16 () =
+  let n1 = Random.bits() in
+  let n2 = n1 lsr 2 in
+  match n1 land 3 with
+  | 0 -> 1 + (n2 land 1)   (* 1-2 *)
+  | 1 -> 3 + (n2 mod 3)    (* 3-4-5 *)
+  | 2 -> 6 + (n2 land 3)   (* 6-7-8-9 *)
+  | 3 -> 10 + (n2 mod 7)   (* 10-16 *)
+  | _ -> assert false
+
+let random_1_32 () =
+  let n1 = Random.bits() in
+  let n2 = n1 lsr 2 in
+  match n1 land 3 with
+  | 0 -> 1 + (n2 land 1)   (* 1-2 *)
+  | 1 -> 3 + (n2 mod 5)    (* 3-4-5-6-7 *)
+  | 2 -> 8 + (n2 mod 8)    (* 8-15 *)
+  | 3 -> 16 + (n2 mod 17)  (* 16-32 *)
+  | _ -> assert false
+
+let random_field () =
+  let (t, w) =
+    match Random.int 9 with
+    | 0   -> (Bool, 1)
+    | 1|2 -> (Char, random_1_8())
+    | 3|4 -> (Short, random_1_16())
+    | _ -> (Int, random_1_32()) in
+  match Random.int 10 with
+  | 0 -> Padding(t, (if Random.int 3 = 0 then 0 else w))
+  | 1 | 2 -> Plain t
+  | _ -> Bitfield(t, w)
+
+let rec random_struct len =
+  if len <= 0 then [] else begin
+    let f = random_field () in
+    f :: random_struct (match f with Padding _ -> len | _ -> len - 1)
+  end
+
+(* Optional filtering of structs where padding fields can increase alignment.
+   ELF says that padding fields are ignored to determine struct alignment,
+   but ARM does otherwise. *)
+
+let alignof = function Bool -> 1 | Char -> 1 | Short -> 2 | Int -> 4
+
+let unstable_alignment str =
+  let rec alignments al_data al_padding = function
+    | [] ->
+        al_padding > al_data
+    | (Plain t | Bitfield(t, _)) :: l ->
+        alignments (max (alignof t) al_data) al_padding l
+    | Padding(t, _) :: l ->
+        alignments al_data (max (alignof t) al_padding) l
+  in
+    alignments 1 1 str
+
+(* Random testing *)
+
+let structsize = ref 4
+let ntests = ref 1000
+let stable = ref false
+
+let _ =
+  Arg.parse [
+     "-size", Arg.Int (fun n -> structsize := n),
+       " <sz> produce structs with <sz> members (default: 4)";
+     "-n", Arg.Int (fun n -> ntests := n),
+       " <num> produce <num> random structs";
+     "-seed", Arg.Int Random.init,
+       " <seed> use the given seed for randomization";
+     "-stable", Arg.Set stable,
+       " don't generate padding fields that could cause differences in alignment"
+  ]
+  (fun s -> raise (Arg.Bad ("don't know what to do with " ^ s)))
+  "Usage: genlayout [options]\n\nOptions are:";
+  for _i = 1 to !ntests do
+    let s = random_struct !structsize in
+    if not (!stable && unstable_alignment s) then begin
+      printf "{\n";
+      c_struct stdout s;
+      printf "TEST%d(%a)\n" !structsize print_struct s;
+      printf "}\n"
+    end
+  done
