test/abi/layout.c
@@ -1,0 +1,59 @@
+#include <stdio.h>
+#include <stdlib.h>
+#include <assert.h>
+#include <string.h>
+#include "../endian.h"
+
+static inline int bit(void * p, unsigned bitno)
+{
+  unsigned byteno = bitno / 8;
+#ifdef ARCH_BIG_ENDIAN
+  unsigned bit_in_byte = 7 - (bitno & 7);
+#else
+  unsigned bit_in_byte = bitno & 7;
+#endif
+  return (((unsigned char *) p)[byteno] >> bit_in_byte) & 1;
+}
+
+void print_prologue(char * name, size_t al, size_t sz)
+{
+  printf("%s: align %d, sizeof %d, layout", name, (int)al, (int)sz);
+}
+
+void print_next_field(_Bool first, size_t sz, void * p)
+{
+  static unsigned pos;
+
+  if (first) pos = 0;
+  /* Find first bit set, starting with [pos] */
+  while (1) {
+    assert (pos < 8 * sz);
+    if (bit(p, pos)) break;
+    pos += 1;
+  }
+  /* Print this position */
+  printf(" %u", pos);
+  /* Skip over one bits */
+  while (pos < 8 * sz && bit(p, pos)) pos++;
+}
+
+void print_epilogue(void)
+{
+  printf("\n");
+}
+
+#define TEST4(s)                                                            \
+  struct s x;                                                               \
+  memset(&x, 0, sizeof(x));                                                 \
+  print_prologue(#s, _Alignof(struct s), sizeof(x));                        \
+  x.a = -1; print_next_field(1, sizeof(x), &x);                             \
+  x.b = -1; print_next_field(0, sizeof(x), &x);                             \
+  x.c = -1; print_next_field(0, sizeof(x), &x);                             \
+  x.d = -1; print_next_field(0, sizeof(x), &x);                             \
+  print_epilogue();
+
+int main()
+{
+#include "layout.h"
+  return 0;
+}
