cfrontend/Initializersproof.v
@@ -12,7 +12,7 @@
 
 (** Compile-time evaluation of initializers for global C variables. *)
 
-Require Import Coqlib Maps.
+Require Import Zwf Coqlib Maps.
 Require Import Errors Integers Floats Values AST Memory Globalenvs Events Smallstep.
 Require Import Ctypes Cop Csyntax Csem.
 Require Import Initializers.
@@ -30,7 +30,7 @@ Variable ge: genv.
 
 Fixpoint simple (a: expr) : Prop :=
   match a with
-  | Eloc _ _ _ => True
+  | Eloc _ _ _ _ => True
   | Evar _ _ => True
   | Ederef r _ => simple r
   | Efield l1 _ _ => simple l1
@@ -65,38 +65,38 @@ Section SIMPLE_EXPRS.
 Variable e: env.
 Variable m: mem.
 
-Inductive eval_simple_lvalue: expr -> block -> ptrofs -> Prop :=
-  | esl_loc: forall b ofs ty,
-      eval_simple_lvalue (Eloc b ofs ty) b ofs
+Inductive eval_simple_lvalue: expr -> block -> ptrofs -> bitfield -> Prop :=
+  | esl_loc: forall b ofs bf ty,
+      eval_simple_lvalue (Eloc b ofs bf ty) b ofs bf
   | esl_var_local: forall x ty b,
       e!x = Some(b, ty) ->
-      eval_simple_lvalue (Evar x ty) b Ptrofs.zero
+      eval_simple_lvalue (Evar x ty) b Ptrofs.zero Full
   | esl_var_global: forall x ty b,
       e!x = None ->
       Genv.find_symbol ge x = Some b ->
-      eval_simple_lvalue (Evar x ty) b Ptrofs.zero
+      eval_simple_lvalue (Evar x ty) b Ptrofs.zero Full
   | esl_deref: forall r ty b ofs,
       eval_simple_rvalue r (Vptr b ofs) ->
-      eval_simple_lvalue (Ederef r ty) b ofs
-  | esl_field_struct: forall r f ty b ofs id co a delta,
+      eval_simple_lvalue (Ederef r ty) b ofs Full
+  | esl_field_struct: forall r f ty b ofs id co a delta bf,
       eval_simple_rvalue r (Vptr b ofs) ->
-      typeof r = Tstruct id a -> ge.(genv_cenv)!id = Some co -> field_offset ge f (co_members co) = OK delta ->
-      eval_simple_lvalue (Efield r f ty) b (Ptrofs.add ofs (Ptrofs.repr delta))
-  | esl_field_union: forall r f ty b ofs id a,
+      typeof r = Tstruct id a -> ge.(genv_cenv)!id = Some co -> field_offset ge f (co_members co) = OK (delta, bf) ->
+      eval_simple_lvalue (Efield r f ty) b (Ptrofs.add ofs (Ptrofs.repr delta)) bf
+  | esl_field_union: forall r f ty b ofs id co a delta bf,
       eval_simple_rvalue r (Vptr b ofs) ->
-      typeof r = Tunion id a ->
-      eval_simple_lvalue (Efield r f ty) b ofs
+      typeof r = Tunion id a -> ge.(genv_cenv)!id = Some co -> union_field_offset ge f (co_members co) = OK (delta, bf) ->
+      eval_simple_lvalue (Efield r f ty) b (Ptrofs.add ofs (Ptrofs.repr delta)) bf
 
 with eval_simple_rvalue: expr -> val -> Prop :=
   | esr_val: forall v ty,
       eval_simple_rvalue (Eval v ty) v
-  | esr_rvalof: forall b ofs l ty v,
-      eval_simple_lvalue l b ofs ->
+  | esr_rvalof: forall b ofs bf l ty v,
+      eval_simple_lvalue l b ofs bf ->
       ty = typeof l ->
-      deref_loc ge ty m b ofs E0 v ->
+      deref_loc ge ty m b ofs bf E0 v ->
       eval_simple_rvalue (Evalof l ty) v
   | esr_addrof: forall b ofs l ty,
-      eval_simple_lvalue l b ofs ->
+      eval_simple_lvalue l b ofs Full ->
       eval_simple_rvalue (Eaddrof l ty) (Vptr b ofs)
   | esr_unop: forall op r1 ty v1 v,
       eval_simple_rvalue r1 v1 ->
@@ -153,7 +153,7 @@ End SIMPLE_EXPRS.
 Definition compat_eval (k: kind) (e: env) (a a': expr) (m: mem) : Prop :=
   typeof a = typeof a' /\
   match k with
-  | LV => forall b ofs, eval_simple_lvalue e m a' b ofs -> eval_simple_lvalue e m a b ofs
+  | LV => forall b ofs bf, eval_simple_lvalue e m a' b ofs bf -> eval_simple_lvalue e m a b ofs bf
   | RV => forall v, eval_simple_rvalue e m a' v -> eval_simple_rvalue e m a v
   end.
 
@@ -167,7 +167,7 @@ Lemma lred_compat:
   forall e l m l' m', lred ge e l m l' m' ->
   m = m' /\ compat_eval LV e l l' m.
 Proof.
-  induction 1; simpl; split; auto; split; auto; intros bx ofsx EV; inv EV.
+  induction 1; simpl; split; auto; split; auto; intros bx ofsx bf' EV; inv EV.
   apply esl_var_local; auto.
   apply esl_var_global; auto.
   constructor. constructor.
@@ -365,6 +365,22 @@ Proof.
   intros. eapply bool_val_inj; eauto. intros. rewrite mem_empty_not_weak_valid_pointer in H2; discriminate.
 Qed.
 
+Lemma add_offset_match:
+  forall v b ofs delta,
+  Val.inject inj v (Vptr b ofs) ->
+  Val.inject inj
+    (if Archi.ptr64
+     then Val.addl v (Vlong (Int64.repr delta))
+     else Val.add v (Vint (Int.repr delta)))
+    (Vptr b (Ptrofs.add ofs (Ptrofs.repr delta))).
+Proof.
+  intros. inv H.
+- rewrite Ptrofs.add_assoc. rewrite (Ptrofs.add_commut (Ptrofs.repr delta0)).
+  unfold Val.addl, Val.add; destruct Archi.ptr64 eqn:SF;
+  econstructor; eauto; rewrite ! Ptrofs.add_assoc; f_equal; f_equal; symmetry; auto with ptrofs.
+- unfold Val.addl, Val.add; destruct Archi.ptr64; auto.
+Qed.
+
 (** Soundness of [constval] with respect to the big-step semantics *)
 
 Lemma constval_rvalue:
@@ -374,20 +390,22 @@ Lemma constval_rvalue:
   constval ge a = OK v' ->
   Val.inject inj v' v
 with constval_lvalue:
-  forall m a b ofs,
-  eval_simple_lvalue empty_env m a b ofs ->
+  forall m a b ofs bf,
+  eval_simple_lvalue empty_env m a b ofs bf ->
   forall v',
   constval ge a = OK v' ->
-  Val.inject inj v' (Vptr b ofs).
+  bf = Full /\ Val.inject inj v' (Vptr b ofs).
 Proof.
   (* rvalue *)
   induction 1; intros vres CV; simpl in CV; try (monadInv CV).
   (* val *)
   destruct v; monadInv CV; constructor.
   (* rval *)
-  inv H1; rewrite H2 in CV; try congruence. eauto. eauto.
+  assert (constval ge l = OK vres) by (destruct (access_mode ty); congruence).
+  exploit constval_lvalue; eauto. intros [A B]. subst bf.
+  inv H1; rewrite H3 in CV; congruence.
   (* addrof *)
-  eauto.
+  eapply constval_lvalue; eauto.
   (* unop *)
   destruct (sem_unary_operation op x (typeof r1) Mem.empty) as [v1'|] eqn:E; inv EQ0.
   exploit (sem_unary_operation_inj inj Mem.empty m).
@@ -438,28 +456,31 @@ Proof.
   (* lvalue *)
   induction 1; intros v' CV; simpl in CV; try (monadInv CV).
   (* var local *)
-  unfold empty_env in H. rewrite PTree.gempty in H. congruence.
+  split; auto. unfold empty_env in H. rewrite PTree.gempty in H. congruence.
   (* var_global *)
-  econstructor. unfold inj. rewrite H0. eauto. auto.
+  split; auto. econstructor. unfold inj. rewrite H0. eauto. auto.
   (* deref *)
-  eauto.
+  split; eauto.
   (* field struct *)
-  rewrite H0 in CV. monadInv CV. unfold lookup_composite in EQ; rewrite H1 in EQ; monadInv EQ.
-  exploit constval_rvalue; eauto. intro MV. inv MV.
-  replace x0 with delta by congruence. rewrite Ptrofs.add_assoc. rewrite (Ptrofs.add_commut (Ptrofs.repr delta0)).
-  simpl; destruct Archi.ptr64 eqn:SF;
-  econstructor; eauto; rewrite ! Ptrofs.add_assoc; f_equal; f_equal; symmetry; auto with ptrofs.
-  destruct Archi.ptr64; auto.
+  rewrite H0 in EQ. monadInv EQ. destruct x0; monadInv EQ2.
+  unfold lookup_composite in EQ0; rewrite H1 in EQ0; monadInv EQ0.
+  exploit constval_rvalue; eauto. intro MV.
+  split. congruence.
+  replace x with delta by congruence.
+  apply (add_offset_match _ _ _ _ MV).
   (* field union *)
-  rewrite H0 in CV. eauto.
+  rewrite H0 in EQ. monadInv EQ. destruct x0; monadInv EQ2.
+  unfold lookup_composite in EQ0; rewrite H1 in EQ0; monadInv EQ0.
+  exploit constval_rvalue; eauto. intro MV.
+  split. congruence.
+  replace x with delta by congruence. 
+  apply (add_offset_match _ _ _ _ MV).
 Qed.
 
 Lemma constval_simple:
   forall a v, constval ge a = OK v -> simple a.
 Proof.
   induction a; simpl; intros vx CV; try (monadInv CV); eauto.
-  destruct (typeof a); discriminate || eauto.
-  monadInv CV. eauto.
   destruct (access_mode ty); discriminate || eauto.
   intuition eauto.
 Qed.
@@ -476,331 +497,757 @@ Proof.
   intros [A [B C]]. intuition. eapply constval_rvalue; eauto.
 Qed.
 
-(** * Relational specification of the translation of initializers *)
+(** * Correctness of operations over the initialization state *)
 
-Definition tr_padding (frm to: Z) : list init_data :=
-  if zlt frm to then Init_space (to - frm) :: nil else nil.
+(** ** Properties of the in-memory bytes denoted by initialization data *)
 
-Inductive tr_init: type -> initializer -> list init_data -> Prop :=
-  | tr_init_sgl: forall ty a d,
-      transl_init_single ge ty a = OK d ->
-      tr_init ty (Init_single a) (d :: nil)
-  | tr_init_arr: forall tyelt nelt attr il d,
-      tr_init_array tyelt il (Z.max 0 nelt) d ->
-      tr_init (Tarray tyelt nelt attr) (Init_array il) d
-  | tr_init_str: forall id attr il co d,
-      lookup_composite ge id = OK co -> co_su co = Struct ->
-      tr_init_struct (Tstruct id attr) (co_members co) il 0 d ->
-      tr_init (Tstruct id attr) (Init_struct il) d
-  | tr_init_uni: forall id attr f i1 co ty1 d,
-      lookup_composite ge id = OK co -> co_su co = Union -> field_type f (co_members co) = OK ty1 ->
-      tr_init ty1 i1 d ->
-      tr_init (Tunion id attr) (Init_union f i1)
-              (d ++ tr_padding (sizeof ge ty1) (sizeof ge (Tunion id attr)))
+Local Notation boid := (Genv.bytes_of_init_data (genv_genv ge)).
+Local Notation boidl := (Genv.bytes_of_init_data_list (genv_genv ge)).
 
-with tr_init_array: type -> initializer_list -> Z -> list init_data -> Prop :=
-  | tr_init_array_nil_0: forall ty,
-      tr_init_array ty Init_nil 0 nil
-  | tr_init_array_nil_pos: forall ty sz,
-      0 < sz ->
-      tr_init_array ty Init_nil sz (Init_space (sz * sizeof ge ty) :: nil)
-  | tr_init_array_cons: forall ty i il sz d1 d2,
-      tr_init ty i d1 -> tr_init_array ty il (sz - 1) d2 ->
-      tr_init_array ty (Init_cons i il) sz (d1 ++ d2)
-
-with tr_init_struct: type -> members -> initializer_list -> Z -> list init_data -> Prop :=
-  | tr_init_struct_nil: forall ty pos,
-      tr_init_struct ty nil Init_nil pos (tr_padding pos (sizeof ge ty))
-  | tr_init_struct_cons: forall ty f1 ty1 fl i1 il pos d1 d2,
-      let pos1 := align pos (alignof ge ty1) in
-      tr_init ty1 i1 d1 ->
-      tr_init_struct ty fl il (pos1 + sizeof ge ty1) d2 ->
-      tr_init_struct ty ((f1, ty1) :: fl) (Init_cons i1 il)
-                     pos (tr_padding pos pos1 ++ d1 ++ d2).
-
-Lemma transl_padding_spec:
-  forall frm to k, padding frm to k = rev (tr_padding frm to) ++ k.
+Lemma boidl_app: forall il2 il1,
+  boidl (il1 ++ il2) = boidl il1 ++ boidl il2.
 Proof.
-  unfold padding, tr_padding; intros. 
-  destruct (zlt frm to); auto.
+  induction il1 as [ | il il1]; simpl. auto. rewrite app_ass. f_equal; auto.
 Qed.
 
-Lemma transl_init_rec_spec:
-  forall i ty k res,
-  transl_init_rec ge ty i k = OK res ->
-  exists d, tr_init ty i d /\ res = rev d ++ k
-
-with transl_init_array_spec:
-  forall il ty sz k res,
-  transl_init_array ge ty il sz k = OK res ->
-  exists d, tr_init_array ty il sz d /\ res = rev d ++ k
-
-with transl_init_struct_spec:
-  forall il ty fl pos k res,
-  transl_init_struct ge ty fl il pos k = OK res ->
-  exists d, tr_init_struct ty fl il pos d /\ res = rev d ++ k.
-
+Corollary boidl_rev_cons: forall i il,
+  boidl (rev il ++ i :: nil) = boidl (rev il) ++ boid i.
 Proof.
-Local Opaque sizeof.
-- destruct i; intros until res; intros TR; simpl in TR.
-+ monadInv TR. exists (x :: nil); split; auto. constructor; auto.
-+ destruct ty; try discriminate.
-  destruct (transl_init_array_spec _ _ _ _ _ TR) as (d & A & B).
-  exists d; split; auto. constructor; auto.
-+ destruct ty; try discriminate. monadInv TR. destruct (co_su x) eqn:SU; try discriminate.
-  destruct (transl_init_struct_spec _ _ _ _ _ _ EQ0) as (d & A & B).
-  exists d; split; auto. econstructor; eauto.
-+ destruct ty; try discriminate.
-  monadInv TR. destruct (co_su x) eqn:SU; monadInv EQ0.
-  destruct (transl_init_rec_spec _ _ _ _ EQ0) as (d & A & B).
-  exists (d ++ tr_padding (sizeof ge x0) (sizeof ge (Tunion i0 a))); split.
-  econstructor; eauto.
-  rewrite rev_app_distr, app_ass, B. apply transl_padding_spec. 
+  intros. rewrite boidl_app. simpl. rewrite <- app_nil_end. auto.
+Qed. 
 
-- destruct il; intros until res; intros TR; simpl in TR.
-+ destruct (zeq sz 0). 
-  inv TR. exists (@nil init_data); split; auto. constructor.
-  destruct (zle 0 sz).
-  inv TR. econstructor; split. constructor. lia. auto.
-  discriminate.
-+ monadInv TR. 
-  destruct (transl_init_rec_spec _ _ _ _ EQ) as (d1 & A1 & B1).
-  destruct (transl_init_array_spec _ _ _ _ _ EQ0) as (d2 & A2 & B2).
-  exists (d1 ++ d2); split. econstructor; eauto. 
-  subst res x. rewrite rev_app_distr, app_ass. auto.
+Definition byte_of_int (n: int) := Byte.repr (Int.unsigned n).
 
-- destruct il; intros until res; intros TR; simpl in TR.
-+ destruct fl; inv TR. econstructor; split. constructor. apply transl_padding_spec.
-+ destruct fl as [ | [f1 ty1] fl ]; monadInv TR.
-  destruct (transl_init_rec_spec _ _ _ _ EQ) as (d1 & A1 & B1).
-  destruct (transl_init_struct_spec _ _ _ _ _ _ EQ0) as (d2 & A2 & B2).
-  exists (tr_padding pos (align pos (alignof ge ty1)) ++ d1 ++ d2); split.
-  econstructor; eauto.
-  rewrite ! rev_app_distr. subst res x. rewrite ! app_ass. rewrite transl_padding_spec. auto.
+Lemma byte_of_int_of_byte: forall b, byte_of_int (int_of_byte b) = b.
+Proof.
+  intros. unfold int_of_byte, byte_of_int.
+  rewrite Int.unsigned_repr, Byte.repr_unsigned. auto.
+  assert(Byte.max_unsigned < Int.max_unsigned) by reflexivity.
+  generalize (Byte.unsigned_range_2 b). lia.
 Qed.
 
-Theorem transl_init_spec:
-  forall ty i d, transl_init ge ty i = OK d -> tr_init ty i d.
+Lemma inj_bytes_1: forall n,
+  inj_bytes (encode_int 1 n) = Byte (Byte.repr n) :: nil.
 Proof.
-  unfold transl_init; intros. monadInv H. 
-  exploit transl_init_rec_spec; eauto. intros (d & A & B). 
-  subst x. unfold rev'; rewrite <- rev_alt. 
-  rewrite rev_app_distr; simpl. rewrite rev_involutive. auto.
+  intros. unfold encode_int, bytes_of_int, rev_if_be. destruct Archi.big_endian; auto.
+Qed.
+
+Lemma inj_bytes_byte: forall b,
+  inj_bytes (encode_int 1 (Int.unsigned (int_of_byte b))) = Byte b :: nil.
+Proof.
+  intros. rewrite inj_bytes_1. do 2 f_equal. apply byte_of_int_of_byte.
+Qed.
+
+Lemma boidl_init_ints8: forall l,
+  boidl (map Init_int8 l) = inj_bytes (map byte_of_int l).
+Proof.
+  induction l as [ | i l]; simpl. auto. rewrite inj_bytes_1; simpl. f_equal; auto.
+Qed.
+
+Lemma boidl_init_bytes: forall l,
+  boidl (map Init_byte l) = inj_bytes l.
+Proof.
+  induction l as [ | b l]; simpl. auto. rewrite inj_bytes_byte, IHl. auto.
+Qed.
+
+Lemma boidl_ints8: forall i n,
+  boidl (repeat (Init_int8 i) n) = repeat (Byte (byte_of_int i)) n.
+Proof.
+  induction n; simpl. auto. rewrite inj_bytes_1. simpl; f_equal; auto.
+Qed.
+
+(** ** Properties of operations over list of initialization data *)
+
+Lemma add_rev_bytes_spec: forall l il,
+  add_rev_bytes l il = List.map Init_byte (List.rev l) ++ il.
+Proof.
+  induction l as [ | b l]; intros; simpl.
+- auto.
+- rewrite IHl. rewrite map_app. simpl. rewrite app_ass. auto.
+Qed.
+
+Lemma add_rev_bytes_spec': forall l il,
+  List.rev (add_rev_bytes l il) = List.rev il ++ List.map Init_byte l.
+Proof.
+  intros. rewrite add_rev_bytes_spec. rewrite rev_app_distr, map_rev, rev_involutive. auto.
+Qed.
+
+Lemma add_zeros_spec: forall n il,
+  0 <= n ->
+  add_zeros n il = List.repeat (Init_int8 Int.zero) (Z.to_nat n) ++ il.
+Proof.
+  intros.
+  unfold add_zeros; rewrite iter_nat_of_Z by auto; rewrite Zabs2Nat.abs_nat_nonneg by auto.
+  induction (Z.to_nat n); simpl. auto. f_equal; auto.
+Qed.
+
+Lemma decompose_spec: forall il depth bl il',
+  decompose il depth = OK (bl, il') ->
+  exists nl, il = List.map Init_int8 nl ++ il'
+          /\ bl = List.map byte_of_int (rev nl)
+          /\ List.length nl = Z.to_nat depth.
+Proof.
+  assert (REC: forall il accu depth bl il',
+               decompose_rec accu il depth = OK (bl, il') ->
+               exists nl, il = List.map Init_int8 nl ++ il'
+                       /\ bl = List.map byte_of_int (rev nl) ++ accu
+                       /\ List.length nl = Z.to_nat depth).
+  { induction il as [ | i il ]; intros until il'; intros D; simpl in D.
+  - destruct (zle depth 0); inv D.
+    exists (@nil int); simpl. rewrite Z_to_nat_neg by auto. auto.
+  - destruct (zle depth 0). 
+    + inv D. exists (@nil int); simpl. rewrite Z_to_nat_neg by auto. auto.
+    + destruct i; try discriminate.
+      apply IHil in D; destruct D as (nl & P & Q & R).
+      exists (i :: nl); simpl; split. congruence. split.
+      rewrite map_app. simpl. rewrite app_ass. exact Q.
+      rewrite R, <- Z2Nat.inj_succ by lia. f_equal; lia.
+  }
+  intros. apply REC in H. destruct H as (nl & P & Q & R). rewrite app_nil_r in Q.
+  exists nl; auto.
+Qed.
+
+Lemma list_repeat_app: forall (A: Type) (a: A) n2 n1,
+  List.repeat a n1 ++ List.repeat a n2 = List.repeat a (n1 + n2)%nat.
+Proof.
+  induction n1; simpl; congruence.
+Qed.
+
+Lemma list_rev_repeat: forall (A: Type) (a: A) n,
+  rev (List.repeat a n) = List.repeat a n.
+Proof.
+  induction n; simpl. auto. rewrite IHn. change (a :: nil) with (repeat a 1%nat).
+  rewrite list_repeat_app. rewrite Nat.add_comm. auto. 
+Qed.
+
+Lemma normalize_boidl: forall il depth il',
+  normalize il depth = OK il' ->
+  boidl (rev il') = boidl (rev il).
+Proof.
+  induction il as [ | i il]; simpl; intros depth il' AT.
+- destruct (zle depth 0); inv AT. auto.
+- destruct (zle depth 0). inv AT. auto.
+  destruct i;
+  try (monadInv AT; simpl;
+       rewrite ? add_rev_bytes_spec', ? boidl_rev_cons, ? boidl_app, ? boidl_init_bytes;
+       erewrite IHil by eauto; reflexivity).
+  set (n := Z.max 0 z) in *. destruct (zle n depth); monadInv AT.
+  + rewrite add_zeros_spec, rev_app_distr, ! boidl_app by lia.
+    erewrite IHil by eauto. f_equal.
+    rewrite list_rev_repeat. simpl. rewrite app_nil_r, boidl_ints8.
+    f_equal. unfold n. apply Z.max_case_strong; intros; auto. rewrite ! Z_to_nat_neg by lia. auto.
+  + rewrite add_zeros_spec, rev_app_distr, !boidl_app by lia.
+    simpl. rewrite boidl_rev_cons, list_rev_repeat. simpl.
+    rewrite app_ass, app_nil_r, !boidl_ints8. f_equal.
+    rewrite list_repeat_app. f_equal. rewrite <- Z2Nat.inj_add by lia.
+    unfold n. apply Z.max_case_strong; intros; f_equal; lia.
+Qed.
+
+Lemma trisection_boidl: forall il depth sz bytes1 bytes2 il',
+  trisection il depth sz = OK (bytes1, bytes2, il') ->
+  boidl (rev il) = boidl (rev il') ++ inj_bytes bytes2 ++ inj_bytes bytes1
+  /\ length bytes1 = Z.to_nat depth
+  /\ length bytes2 = Z.to_nat sz.
+Proof.
+  unfold trisection; intros. monadInv H.
+  apply normalize_boidl in EQ. rewrite <- EQ.
+  apply decompose_spec in EQ1. destruct EQ1 as (nl1 & A1 & B1 & C1).
+  apply decompose_spec in EQ0. destruct EQ0 as (nl2 & A2 & B2 & C2).
+  split.
+- rewrite A1, A2, !rev_app_distr, !boidl_app, app_ass.
+  rewrite <- !map_rev, !boidl_init_ints8. rewrite <- B1, <- B2. auto.
+- rewrite B1, B2, !map_length, !rev_length. auto.
+Qed. 
+
+Lemma store_init_data_loadbytes:
+  forall m b p i m',
+  Genv.store_init_data ge m b p i = Some m' ->
+  match i with Init_space _ => False | _ => True end ->
+  Mem.loadbytes m' b p (init_data_size i) = Some (boid i).
+Proof.
+  intros; destruct i; simpl in H; try apply (Mem.loadbytes_store_same _ _ _ _ _ _ H).
+- contradiction.
+- rewrite Genv.init_data_size_addrof. simpl.
+  destruct (Genv.find_symbol ge i) as [b'|]; try discriminate.
+  rewrite (Mem.loadbytes_store_same _ _ _ _ _ _ H).
+  unfold encode_val, Mptr; destruct Archi.ptr64; reflexivity.
+Qed.
+
+(** ** Validity and size of initialization data *)
+
+Definition idvalid (i: init_data) : Prop :=
+  match i with
+  | Init_addrof symb ofs => exists b, Genv.find_symbol ge symb = Some b
+  | _ => True
+  end.
+
+Fixpoint idlvalid (p: Z) (il: list init_data) {struct il} : Prop :=
+  match il with
+  | nil => True
+  | i1 :: il =>
+        (Genv.init_data_alignment i1 | p)
+     /\ idvalid i1
+     /\ idlvalid (p + init_data_size i1) il
+  end.
+
+Lemma idlvalid_app: forall l2 l1 pos,
+  idlvalid pos (l1 ++ l2) <-> idlvalid pos l1 /\ idlvalid (pos + init_data_list_size l1) l2.
+Proof.
+  induction l1 as [ | d l1]; intros; simpl.
+- rewrite Z.add_0_r; tauto.
+- rewrite IHl1. rewrite Z.add_assoc. tauto.
+Qed.
+
+Lemma add_rev_bytes_valid: forall il bl,
+  idlvalid 0 (rev il) -> idlvalid 0 (rev (add_rev_bytes bl il)).
+Proof.
+  intros. rewrite add_rev_bytes_spec, rev_app_distr, idlvalid_app. split; auto.
+  generalize (rev bl) (0 + init_data_list_size (rev il)). induction l; simpl; intros.
+  auto.
+  rewrite idlvalid_app; split; auto. simpl. auto using Z.divide_1_l.
+Qed.
+
+Lemma add_zeros_valid: forall il n,
+  0 <= n -> idlvalid 0 (rev il) -> idlvalid 0 (rev (add_zeros n il)).
+Proof.
+  intros. rewrite add_zeros_spec, rev_app_distr, idlvalid_app by auto.
+  split; auto.
+  generalize (Z.to_nat n) (0 + init_data_list_size (rev il)). induction n0; simpl; intros.
+  auto.
+  rewrite idlvalid_app; split; auto. simpl. auto using Z.divide_1_l.
+Qed.
+
+Lemma normalize_valid: forall il depth il',
+  normalize il depth = OK il' -> idlvalid 0 (rev il) -> idlvalid 0 (rev il').
+Proof.
+  induction il as [ | i il]; simpl; intros.
+- destruct (zle depth 0); inv H. simpl. tauto.
+- destruct (zle depth 0). inv H. auto.
+  rewrite idlvalid_app in H0; destruct H0.
+  destruct i; try (monadInv H; apply add_rev_bytes_valid; eapply IHil; eauto).
+  + monadInv H. simpl. rewrite idlvalid_app; split. eauto. simpl; auto using Z.divide_1_l. 
+  + destruct (zle (Z.max 0 z)); monadInv H.
+    * apply add_zeros_valid. lia. eauto.
+    * apply add_zeros_valid. lia. simpl. rewrite idlvalid_app; split. auto. simpl; auto using Z.divide_1_l.
+Qed.
+
+Lemma trisection_valid: forall il depth sz bytes1 bytes2 il',
+  trisection il depth sz = OK (bytes1, bytes2, il') ->
+  idlvalid 0 (rev il) ->
+  idlvalid 0 (rev il').
+Proof.
+  unfold trisection; intros. monadInv H.
+  apply decompose_spec in EQ1. destruct EQ1 as (nl1 & A1 & B1 & C1).
+  apply decompose_spec in EQ0. destruct EQ0 as (nl2 & A2 & B2 & C2).
+  exploit normalize_valid; eauto. rewrite A1, A2, !rev_app_distr, !idlvalid_app.
+  tauto.
+Qed.
+
+Lemma init_data_size_boid: forall i,
+  init_data_size i = Z.of_nat (length (boid i)).
+Proof.
+  intros. destruct i; simpl; rewrite ?length_inj_bytes, ?encode_int_length; auto.
+- rewrite repeat_length. rewrite Z_to_nat_max; auto.
+- destruct (Genv.find_symbol ge i), Archi.ptr64; reflexivity.
+Qed.
+
+Lemma init_data_list_size_boidl: forall il,
+  init_data_list_size il = Z.of_nat (length (boidl il)).
+Proof.
+  induction il as [ | i il]; simpl. auto. 
+  rewrite app_length, init_data_size_boid. lia.
+Qed.
+
+Lemma init_data_list_size_app: forall l1 l2,
+  init_data_list_size (l1 ++ l2) = init_data_list_size l1 + init_data_list_size l2.
+Proof.
+  induction l1 as [ | i l1]; intros; simpl. auto. rewrite IHl1; lia.
+Qed.
+
+(** ** Memory areas that are initialized to zeros *)
+
+Definition reads_as_zeros (m: mem) (b: block) (from to: Z) : Prop :=
+  forall i, from <= i < to -> Mem.loadbytes m b i 1 = Some (Byte Byte.zero :: nil).
+
+Lemma reads_as_zeros_mono: forall m b from1 from2 to1 to2,
+  reads_as_zeros m b from1 to1 -> from1 <= from2 -> to2 <= to1 ->
+  reads_as_zeros m b from2 to2.
+Proof.
+  intros; red; intros. apply H; lia.
+Qed.
+
+Remark reads_as_zeros_unchanged:
+  forall (P: block -> Z -> Prop) m b from to m',
+  reads_as_zeros m b from to ->
+  Mem.unchanged_on P m m' ->
+  (forall i, from <= i < to -> P b i) ->
+  reads_as_zeros m' b from to.
+Proof.
+  intros; red; intros. eapply Mem.loadbytes_unchanged_on; eauto.
+  intros; apply H1. lia.
+Qed.
+
+Lemma reads_as_zeros_loadbytes: forall m b from to,
+  reads_as_zeros m b from to ->
+  forall len pos, from <= pos -> pos + len <= to -> 0 <= len ->
+  Mem.loadbytes m b pos len = Some (repeat (Byte Byte.zero) (Z.to_nat len)).
+Proof.
+  intros until to; intros RZ.
+  induction len using (well_founded_induction (Zwf_well_founded 0)).
+  intros. destruct (zeq len 0).
+- subst len. rewrite Mem.loadbytes_empty by lia. auto.
+- replace (Z.to_nat len) with (S (Z.to_nat (len - 1))).
+  change (repeat (Byte Byte.zero) (S (Z.to_nat (len - 1))))
+    with ((Byte Byte.zero :: nil) ++ repeat (Byte Byte.zero) (Z.to_nat (len - 1))).
+  replace len with (1 + (len - 1)) at 1 by lia. 
+  apply Mem.loadbytes_concat; try lia.
+  + apply RZ. lia.
+  + apply H; unfold Zwf; lia.
+  + rewrite <- Z2Nat.inj_succ by lia. f_equal; lia. 
+Qed.
+
+Lemma reads_as_zeros_equiv: forall m b from to,
+  reads_as_zeros m b from to <-> Genv.readbytes_as_zero m b from (to - from).
+Proof.
+  intros; split; intros.
+- red; intros. set (len := Z.of_nat n).
+  replace n with (Z.to_nat len) by apply Nat2Z.id.
+  eapply reads_as_zeros_loadbytes; eauto. lia. lia.
+- red; intros. red in H. apply (H i 1%nat). lia. lia.
+Qed.
+
+(** ** Semantic correctness of state operations *)
+
+(** Semantic interpretation of states. *)
+
+Record match_state (s: state) (m: mem) (b: block) : Prop := {
+  match_range:
+    0 <= s.(curr) <= s.(total_size);
+  match_contents:
+    Mem.loadbytes m b 0 s.(curr) = Some (boidl (rev s.(init)));
+  match_valid:
+    idlvalid 0 (rev s.(init));
+  match_uninitialized:
+    reads_as_zeros m b s.(curr) s.(total_size)
+}.
+
+Lemma match_size: forall s m b,
+  match_state s m b ->
+  init_data_list_size (rev s.(init)) = s.(curr).
+Proof.
+  intros. rewrite init_data_list_size_boidl.
+  erewrite Mem.loadbytes_length by (eapply match_contents; eauto).
+  apply Z2Nat.id. eapply match_range; eauto.
+Qed.
+
+Lemma curr_pad_to: forall s pos,
+  curr s <= curr (pad_to s pos) /\ pos <= curr (pad_to s pos).
+Proof.
+  unfold pad_to; intros. destruct (zle pos (curr s)); simpl; lia.
+Qed.
+
+Lemma total_size_pad_to: forall s pos,
+  total_size (pad_to s pos) = total_size s.
+Proof.
+  unfold pad_to; intros. destruct (zle pos (curr s)); auto.
+Qed.
+
+Lemma pad_to_correct: forall pos s m b,
+  match_state s m b -> pos <= s.(total_size) ->
+  match_state (pad_to s pos) m b.
+Proof.
+  intros. unfold pad_to. destruct (zle pos (curr s)); auto.
+  destruct H; constructor; simpl; intros.
+- lia.
+- rewrite boidl_rev_cons. simpl.
+  replace pos with (s.(curr) + (pos - s.(curr))) at 1 by lia.
+  apply Mem.loadbytes_concat; try lia.
+    * auto.
+    * eapply reads_as_zeros_loadbytes; eauto. lia. lia. lia.
+- rewrite idlvalid_app. split; auto. simpl. intuition auto using Z.divide_1_l.
+- eapply reads_as_zeros_mono; eauto; lia.
+Qed.
+
+Lemma trisection_correct: forall s m b pos sz bytes1 bytes2 il,
+  match_state s m b ->
+  trisection s.(init) (s.(curr) - (pos + sz)) sz = OK (bytes1, bytes2, il) ->
+  0 <= pos -> pos + sz <= s.(curr) -> 0 <= sz ->
+  Mem.loadbytes m b 0 pos = Some (boidl (rev il))
+  /\ Mem.loadbytes m b pos sz = Some (inj_bytes bytes2)
+  /\ Mem.loadbytes m b (pos + sz) (s.(curr) - (pos + sz)) = Some (inj_bytes bytes1).
+Proof.
+  intros. apply trisection_boidl in H0. destruct H0 as (A & B & C).
+  set (depth := curr s - (pos + sz)) in *.
+  pose proof (match_contents _ _ _ H) as D.
+  replace (curr s) with ((pos + sz) + depth) in D by lia.
+  exploit Mem.loadbytes_split. eexact D. lia. lia.
+  rewrite Z.add_0_l. intros (bytes0 & bytes1' & LB0 & LB1 & E1).
+  exploit Mem.loadbytes_split. eexact LB0. lia. lia.
+  rewrite Z.add_0_l. intros (bytes3 & bytes2' & LB3 & LB2 & E2).
+  rewrite A in E1. rewrite <- app_ass in E1.
+  exploit list_append_injective_r. eexact E1.
+  { unfold inj_bytes; rewrite map_length. erewrite Mem.loadbytes_length; eauto. }
+  intros (E3 & E4).
+  rewrite E2 in E3.
+  exploit list_append_injective_r. eexact E3.
+  { unfold inj_bytes; rewrite map_length. erewrite Mem.loadbytes_length; eauto. }
+  intros (E5 & E6).
+  intuition congruence.
+Qed.
+
+Remark decode_int_zero_ext: forall n bytes,
+  0 <= n <= 4 -> n = Z.of_nat (length bytes) ->
+  Int.zero_ext (n * 8) (Int.repr (decode_int bytes)) = Int.repr (decode_int bytes).
+Proof.
+  intros.
+  assert (0 <= decode_int bytes < two_p (n * 8)).
+  { rewrite H0. replace (length bytes) with (length (rev_if_be bytes)). 
+    apply int_of_bytes_range.
+    apply rev_if_be_length. }
+  assert (two_p (n * 8) <= Int.modulus).
+  { apply (two_p_monotone (n * 8) 32); lia. } 
+  unfold Int.zero_ext.
+  rewrite Int.unsigned_repr by (unfold Int.max_unsigned; lia).
+  rewrite Zbits.Zzero_ext_mod by lia.
+  rewrite Zmod_small by auto. auto.
+Qed.
+
+Theorem load_int_correct: forall s m b pos isz i v,
+  match_state s m b ->
+  load_int s pos isz = OK i ->
+  Mem.load (chunk_for_carrier isz) m b pos = Some v ->
+  v = Vint i.
+Proof.
+  intros until v; intros MS RI LD.
+  exploit Mem.load_valid_access. eauto. intros [PERM ALIGN].
+  unfold load_int in RI. 
+  set (chunk := chunk_for_carrier isz) in *.
+  set (sz := size_chunk chunk) in *.
+  assert (sz > 0) by (apply size_chunk_pos).
+  set (s1 := pad_to s (pos + sz)) in *.
+  assert (pos + sz <= curr s1) by (apply curr_pad_to).
+  monadInv RI. InvBooleans. destruct x as [[bytes1 bytes2] il].
+  assert (MS': match_state s1 m b) by (apply pad_to_correct; auto).
+  exploit trisection_correct; eauto. lia.
+  intros (L1 & L2 & L3).
+  assert (LEN: Z.of_nat (length bytes2) = sz).
+  { apply Mem.loadbytes_length in L2. unfold inj_bytes in L2.
+    rewrite map_length in L2. rewrite L2. apply Z2Nat.id; lia. }
+  exploit Mem.loadbytes_load. eexact L2. exact ALIGN. rewrite LD. 
+  unfold decode_val. rewrite proj_inj_bytes. intros E; inv E; inv EQ0.
+  unfold chunk, chunk_for_carrier; destruct isz; f_equal.
+  - apply (decode_int_zero_ext 1). lia. auto.
+  - apply (decode_int_zero_ext 2). lia. auto.
+  - apply (decode_int_zero_ext 1). lia. auto.
+Qed.
+
+Remark loadbytes_concat_3: forall m b ofs1 len1 l1 ofs2 len2 l2 ofs3 len3 l3 len,
+  Mem.loadbytes m b ofs1 len1 = Some l1 ->
+  Mem.loadbytes m b ofs2 len2 = Some l2 ->
+  Mem.loadbytes m b ofs3 len3 = Some l3 ->
+  ofs2 = ofs1 + len1 -> ofs3 = ofs2 + len2 -> 0 <= len1 -> 0 <= len2 -> 0 <= len3 ->
+  len = len1 + len2 + len3 ->
+  Mem.loadbytes m b ofs1 len = Some (l1 ++ l2 ++ l3).
+Proof.
+  intros. rewrite H7, <- Z.add_assoc. apply Mem.loadbytes_concat. auto.
+  apply Mem.loadbytes_concat. rewrite <- H2; auto. rewrite <- H2, <- H3; auto.
+  lia. lia. lia. lia.
+Qed. 
+
+Theorem store_data_correct: forall s m b pos i s' m',
+  match_state s m b ->
+  store_data s pos i = OK s' ->
+  Genv.store_init_data ge m b pos i = Some m' ->
+  match i with Init_space _ => False | _ => True end ->
+  match_state s' m' b.
+Proof.
+  intros until m'; intros MS ST SI NOSPACE.
+  exploit Genv.store_init_data_aligned; eauto. intros ALIGN.
+  assert (VALID: idvalid i).
+  { destruct i; simpl; auto. simpl in SI. destruct (Genv.find_symbol ge i); try discriminate. exists b0; auto. }
+  unfold store_data in ST.
+  set (sz := init_data_size i) in *.
+  assert (sz >= 0) by (apply init_data_size_pos).
+  set (s1 := pad_to s (pos + sz)) in *.
+  monadInv ST. InvBooleans.
+  assert (U: Mem.unchanged_on (fun b i => ~(pos <= i < pos + sz)) m m').
+  { eapply Genv.store_init_data_unchanged. eauto. tauto. }
+  exploit store_init_data_loadbytes; eauto. fold sz. intros D.
+  destruct (zle (curr s) pos).
+- inv ST.
+  set (il := if zlt (curr s) pos then Init_space (pos - curr s) :: init s else init s).
+  assert (IL: boidl (rev il) = boidl (rev (init s)) ++ repeat (Byte Byte.zero) (Z.to_nat (pos - curr s))).
+  { unfold il; destruct (zlt (curr s) pos).
+  - simpl rev. rewrite boidl_rev_cons. simpl. auto.
+  - rewrite Z_to_nat_neg by lia. simpl. rewrite app_nil_r; auto.
+  }
+  constructor; simpl; intros.
+  + lia.
+  + rewrite boidl_rev_cons, IL, app_ass.
+    apply loadbytes_concat_3 with (len1 := curr s) (ofs2 := curr s) (len2 := pos - curr s) (ofs3 := pos) (len3 := sz); try lia.
+    * eapply Mem.loadbytes_unchanged_on; eauto.
+      intros. simpl. lia.
+      eapply match_contents; eauto.
+    * eapply Mem.loadbytes_unchanged_on; eauto.
+      intros. simpl. lia.
+      eapply reads_as_zeros_loadbytes. eapply match_uninitialized; eauto. lia. lia. lia.
+    * exact D.
+    * eapply match_range; eauto.
+  + rewrite idlvalid_app; split.
+    * unfold il; destruct (zlt (curr s) pos).
+      ** simpl; rewrite idlvalid_app; split. eapply match_valid; eauto. simpl. auto using Z.divide_1_l.
+      ** eapply match_valid; eauto.
+    * simpl.
+      replace (init_data_list_size (rev il)) with pos. tauto.
+      unfold il; destruct (zlt (curr s) pos).
+      ** simpl; rewrite init_data_list_size_app; simpl.
+         erewrite match_size by eauto. lia.
+      ** erewrite match_size by eauto. lia.
+  + eapply reads_as_zeros_unchanged; eauto.
+    eapply reads_as_zeros_mono. eapply match_uninitialized; eauto. lia. lia.
+    intros. simpl. lia.
+- monadInv ST. destruct x as [[bytes1 bytes2] il]. inv EQ0.
+  assert (pos + sz <= curr s1) by (apply curr_pad_to).
+  assert (MS': match_state s1 m b) by (apply pad_to_correct; auto).
+  exploit trisection_correct; eauto. lia.
+  intros (L1 & L2 & L3).
+  constructor; simpl; intros.
+  + eapply match_range; eauto.
+  + rewrite add_rev_bytes_spec, rev_app_distr; simpl; rewrite app_ass; simpl.
+    rewrite <- map_rev, rev_involutive.
+    rewrite boidl_app. simpl. rewrite boidl_init_bytes.
+    apply loadbytes_concat_3 with (len1 := pos) (ofs2 := pos) (len2 := sz) (ofs3 := pos + sz)
+                                  (len3 := curr s1 - (pos + sz)); try lia.
+    * eapply Mem.loadbytes_unchanged_on; eauto.
+      intros. simpl. lia.
+    * exact D.
+    * eapply Mem.loadbytes_unchanged_on; eauto.
+      intros. simpl. lia.
+  + apply add_rev_bytes_valid. simpl; rewrite idlvalid_app; split.
+    * eapply trisection_valid; eauto. eapply match_valid; eauto.
+    * rewrite init_data_list_size_boidl. erewrite Mem.loadbytes_length by eauto.
+      rewrite Z2Nat.id by lia. simpl. tauto.
+  + eapply reads_as_zeros_unchanged; eauto. eapply match_uninitialized; eauto.
+    intros. simpl. lia.
+Qed.
+
+Corollary store_int_correct: forall s m b pos isz n s' m',
+  match_state s m b ->
+  store_int s pos isz n = OK s' ->
+  Mem.store (chunk_for_carrier isz) m b pos (Vint n) = Some m' ->
+  match_state s' m' b.
+Proof.
+  intros. eapply store_data_correct; eauto.
+- destruct isz; exact H1.
+- destruct isz; exact I.
+Qed.
+
+Theorem init_data_list_of_state_correct: forall s m b il b' m1,
+  match_state s m b ->
+  init_data_list_of_state s = OK il ->
+  Mem.range_perm m1 b' 0 s.(total_size) Cur Writable ->
+  reads_as_zeros m1 b' 0 s.(total_size) ->
+  exists m2,
+     Genv.store_init_data_list ge m1 b' 0 il = Some m2
+  /\ Mem.loadbytes m2 b' 0 (init_data_list_size il) = Mem.loadbytes m b 0 s.(total_size).
+Proof.
+  intros. unfold init_data_list_of_state in H0; monadInv H0. rename l into LE.
+  set (s1 := pad_to s s.(total_size)) in *.
+  assert (MS1: match_state s1 m b) by (apply pad_to_correct; auto; lia).
+  apply reads_as_zeros_equiv in H2. rewrite Z.sub_0_r in H2.
+  assert (R: rev' (init s1) = rev (init s1)).
+  { unfold rev'. rewrite <- rev_alt. auto. }
+  assert (C: curr s1 = total_size s).
+  { unfold s1, pad_to. destruct zle; simpl; lia. }
+  assert (A: Genv.init_data_list_aligned 0 (rev (init s1))).
+  { exploit match_valid; eauto. generalize (rev (init s1)) 0.
+    induction l as [ | i l]; simpl; intuition. }
+  assert (B: forall id ofs, In (Init_addrof id ofs) (rev (init s1)) ->
+             exists b, Genv.find_symbol ge id = Some b).
+  { intros id ofs. exploit match_valid; eauto. generalize (rev (init s1)) 0.
+    induction l as [ | i l]; simpl; intuition eauto. subst i; assumption. }
+  exploit Genv.store_init_data_list_exists.
+  2: eexact A. 2: eexact B.
+  erewrite match_size by eauto. rewrite C. eauto.
+  intros (m2 & ST). exists m2; split.
+- rewrite R. auto.
+- rewrite R. transitivity (Some (boidl (rev (init s1)))).
+  + eapply Genv.store_init_data_list_loadbytes; eauto.
+    erewrite match_size, C by eauto. auto.
+  + symmetry. rewrite <- C. eapply match_contents; eauto.
+Qed.
+
+(** ** Total size properties *)
+
+Lemma total_size_store_data: forall s pos i s',
+  store_data s pos i = OK s' -> total_size s' = total_size s.
+Proof.
+  unfold store_data; intros. monadInv H. destruct (zle (curr s) pos); monadInv H.
+- auto.
+- destruct x as [[bytes1 bytes2] il2]. inv EQ0. simpl. apply total_size_pad_to.
+Qed.
+
+Lemma total_size_transl_init_bitfield: forall ce s ty sz p w i pos s',
+  transl_init_bitfield ce s ty sz p w i pos = OK s' -> total_size s' = total_size s.
+Proof.
+  unfold transl_init_bitfield; intros. destruct i; monadInv H. destruct x; monadInv EQ0.
+  eapply total_size_store_data. eexact EQ2.
+Qed.
+
+Lemma total_size_transl_init_rec: forall ce s ty i pos s',
+  transl_init_rec ce s ty i pos = OK s' -> total_size s' = total_size s
+with total_size_transl_init_array: forall ce s tyelt il pos s',
+  transl_init_array ce s tyelt il pos = OK s' -> total_size s' = total_size s
+with total_size_transl_init_struct: forall ce s ms il base pos s',
+  transl_init_struct ce s ms il base pos = OK s' -> total_size s' = total_size s.
+Proof.
+- destruct i; simpl; intros.
+  + monadInv H; eauto using total_size_store_data.
+  + destruct ty; monadInv H. eauto.
+  + destruct ty; monadInv H. destruct (co_su x); try discriminate. eauto.
+  + destruct ty; monadInv H. destruct (co_su x); monadInv EQ0. destruct x2.
+    * eauto.
+    * eauto using total_size_transl_init_bitfield.
+- destruct il; simpl; intros.
+  + inv H; auto.
+  + monadInv H. transitivity (total_size x); eauto.
+- destruct il; simpl; intros.
+  + inv H; auto.
+  + revert ms pos H. induction ms; intros.
+    * inv H.
+    * destruct (member_not_initialized a). eapply IHms; eauto.
+      monadInv H. transitivity (total_size x1). eauto.
+      destruct x0; eauto using total_size_transl_init_bitfield.
 Qed.
 
 (** * Soundness of the translation of initializers *)
 
 (** Soundness for single initializers. *)
 
-Theorem transl_init_single_steps:
-  forall ty a data f m v1 ty1 m' v chunk b ofs m'',
+Inductive exec_assign: mem -> block -> Z -> bitfield -> type -> val -> mem -> Prop :=
+  | exec_assign_full: forall m b ofs ty v m' chunk,
+      access_mode ty = By_value chunk ->
+      Mem.store chunk m b ofs v = Some m' ->
+      exec_assign m b ofs Full ty v m'
+  | exec_assign_bits: forall m b ofs sz sg sg1 attr pos width ty n m' c,
+      type_is_volatile ty = false ->
+      0 <= pos -> 0 < width -> pos + width <= bitsize_intsize sz ->
+      sg1 = (if zlt width (bitsize_intsize sz) then Signed else sg) ->
+      Mem.load (chunk_for_carrier sz) m b ofs = Some (Vint c) ->
+      Mem.store (chunk_for_carrier sz) m b ofs
+                (Vint (Int.bitfield_insert (first_bit sz pos width) width c n)) = Some m' ->
+      exec_assign m b ofs (Bits sz sg pos width) (Tint sz sg1 attr) (Vint n) m'.
+
+Lemma transl_init_single_sound:
+  forall ty a data f m v1 ty1 m' v b ofs m'',
   transl_init_single ge ty a = OK data ->
   star step ge (ExprState f a Kstop empty_env m) E0 (ExprState f (Eval v1 ty1) Kstop empty_env m') ->
   sem_cast v1 ty1 ty m' = Some v ->
-  access_mode ty = By_value chunk ->
-  Mem.store chunk m' b ofs v = Some m'' ->
-  Genv.store_init_data ge m b ofs data = Some m''.
+  exec_assign m' b ofs Full ty v m'' ->
+  Genv.store_init_data ge m b ofs data = Some m''
+  /\ match data with Init_space _ => False | _ => True end.
 Proof.
-  intros. monadInv H. monadInv EQ. 
+  intros until m''; intros TR STEPS CAST ASG.
+  monadInv TR. monadInv EQ. 
   exploit constval_steps; eauto. intros [A [B C]]. subst m' ty1.
   exploit sem_cast_match; eauto. intros D.
-  unfold Genv.store_init_data.
-  inv D.
+  inv ASG. rename H into A. unfold Genv.store_init_data. inv D.
 - (* int *)
   remember Archi.ptr64 as ptr64.  destruct ty; try discriminate EQ0.
 + destruct i0; inv EQ0.
-  destruct s; simpl in H2; inv H2. rewrite <- Mem.store_signed_unsigned_8; auto. auto.
-  destruct s; simpl in H2; inv H2. rewrite <- Mem.store_signed_unsigned_16; auto. auto.
-  simpl in H2; inv H2. assumption.
-  simpl in H2; inv H2. assumption.
-+ destruct ptr64; inv EQ0. simpl in H2; unfold Mptr in H2; rewrite <- Heqptr64 in H2; inv H2. assumption.
+  destruct s; simpl in A; inv A. rewrite <- Mem.store_signed_unsigned_8; auto. auto.
+  destruct s; simpl in A; inv A. rewrite <- Mem.store_signed_unsigned_16; auto. auto.
+  simpl in A; inv A. auto.
+  simpl in A; inv A. auto.
++ destruct ptr64; inv EQ0. simpl in A; unfold Mptr in A; rewrite <- Heqptr64 in A; inv A. auto.
 - (* Long *)
-  remember Archi.ptr64 as ptr64. destruct ty; inv EQ0.
-+ simpl in H2; inv H2. assumption.
-+ simpl in H2; unfold Mptr in H2; destruct Archi.ptr64; inv H4. 
-  inv H2; assumption.
+  remember Archi.ptr64 as ptr64. destruct ty; monadInv EQ0.
++ simpl in A; inv A. auto.
++ simpl in A; unfold Mptr in A; rewrite <- Heqptr64 in A; inv A. auto.
 - (* float *)
   destruct ty; try discriminate.
-  destruct f1; inv EQ0; simpl in H2; inv H2; assumption.
+  destruct f1; inv EQ0; simpl in A; inv A; auto.
 - (* single *)
   destruct ty; try discriminate.
-  destruct f1; inv EQ0; simpl in H2; inv H2; assumption.
+  destruct f1; inv EQ0; simpl in A; inv A; auto.
 - (* pointer *)
   unfold inj in H.
-  assert (data = Init_addrof b1 ofs1 /\ chunk = Mptr).
+  assert (X: data = Init_addrof b1 ofs1 /\ chunk = Mptr).
   { remember Archi.ptr64 as ptr64.
     destruct ty; inversion EQ0.
-    destruct i; inv H5. unfold Mptr. destruct Archi.ptr64; inv H6; inv H2; auto.
-    subst ptr64. unfold Mptr. destruct Archi.ptr64; inv H5; inv H2; auto.
-    inv H2. auto. }
-  destruct H4; subst. destruct (Genv.find_symbol ge b1); inv H.
-  rewrite Ptrofs.add_zero in H3. auto.
+    - destruct i; monadInv H2. unfold Mptr. rewrite <- Heqptr64. inv A; auto.
+    - monadInv H2. unfold Mptr. rewrite <- Heqptr64. inv A; auto.
+    - inv A; auto.
+  }
+  destruct X; subst. destruct (Genv.find_symbol ge b1); inv H.
+  rewrite Ptrofs.add_zero in H0. auto.
 - (* undef *)
   discriminate.
 Qed.
 
-(** Size properties for initializers. *)
-
-Lemma transl_init_single_size:
-  forall ty a data,
-  transl_init_single ge ty a = OK data ->
-  init_data_size data = sizeof ge ty.
-Proof.
-  intros. monadInv H. monadInv EQ. remember Archi.ptr64 as ptr64. destruct x.
-- monadInv EQ0.
-- destruct ty; try discriminate.
-  destruct i0; inv EQ0; auto.
-  destruct ptr64; inv EQ0. 
-Local Transparent sizeof.
-  unfold sizeof. rewrite <- Heqptr64; auto.
-- destruct ty; inv EQ0; auto. 
-  unfold sizeof. destruct Archi.ptr64; inv H0; auto.
-- destruct ty; try discriminate.
-  destruct f0; inv EQ0; auto.
-- destruct ty; try discriminate.
-  destruct f0; inv EQ0; auto.
-- destruct ty; try discriminate.
-  destruct i0; inv EQ0; auto.
-  destruct Archi.ptr64 eqn:SF; inv H0. simpl. rewrite SF; auto.
-  destruct ptr64; inv EQ0. simpl. rewrite <- Heqptr64; auto.
-  inv EQ0. unfold init_data_size, sizeof. auto.
-Qed.
-
-Notation idlsize := init_data_list_size.
-
-Remark padding_size:
-  forall frm to, frm <= to -> idlsize (tr_padding frm to) = to - frm.
-Proof.
-  unfold tr_padding; intros. destruct (zlt frm to).
-  simpl. extlia.
-  simpl. lia.
-Qed.
-
-Remark idlsize_app:
-  forall d1 d2, idlsize (d1 ++ d2) = idlsize d1 + idlsize d2.
-Proof.
-  induction d1; simpl; intros.
-  auto.
-  rewrite IHd1. lia.
-Qed.
-
-Remark union_field_size:
-  forall f ty fl, field_type f fl = OK ty -> sizeof ge ty <= sizeof_union ge fl.
-Proof.
-  induction fl as [|[i t]]; simpl; intros.
-- inv H.
-- destruct (ident_eq f i).
-  + inv H. extlia.
-  + specialize (IHfl H). extlia.
-Qed.
-
-Hypothesis ce_consistent: composite_env_consistent ge.
-
-Lemma tr_init_size:
-  forall i ty data,
-  tr_init ty i data ->
-  idlsize data = sizeof ge ty
-with tr_init_array_size:
-  forall ty il sz data,
-  tr_init_array ty il sz data ->
-  idlsize data = sizeof ge ty * sz
-with tr_init_struct_size:
-  forall ty fl il pos data,
-  tr_init_struct ty fl il pos data ->
-  sizeof_struct ge pos fl <= sizeof ge ty ->
-  idlsize data + pos = sizeof ge ty.
-Proof.
-Local Opaque sizeof.
-- destruct 1; simpl.
-+ erewrite transl_init_single_size by eauto. lia.
-+ Local Transparent sizeof. simpl. eapply tr_init_array_size; eauto. 
-+ replace (idlsize d) with (idlsize d + 0) by lia.
-  eapply tr_init_struct_size; eauto. simpl.
-  unfold lookup_composite in H. destruct (ge.(genv_cenv)!id) as [co'|] eqn:?; inv H.
-  erewrite co_consistent_sizeof by (eapply ce_consistent; eauto).
-  unfold sizeof_composite. rewrite H0. apply align_le.
-  destruct (co_alignof_two_p co) as [n EQ]. rewrite EQ. apply two_power_nat_pos.
-+ rewrite idlsize_app, padding_size. 
-  exploit tr_init_size; eauto. intros EQ; rewrite EQ. lia.
-  simpl. unfold lookup_composite in H. destruct (ge.(genv_cenv)!id) as [co'|] eqn:?; inv H.
-  apply Z.le_trans with (sizeof_union ge (co_members co)).
-  eapply union_field_size; eauto.
-  erewrite co_consistent_sizeof by (eapply ce_consistent; eauto).
-  unfold sizeof_composite. rewrite H0. apply align_le.
-  destruct (co_alignof_two_p co) as [n EQ]. rewrite EQ. apply two_power_nat_pos.
-
-- destruct 1; simpl.
-+ lia.
-+ rewrite Z.mul_comm.
-  assert (0 <= sizeof ge ty * sz).
-  { apply Zmult_gt_0_le_0_compat. lia. generalize (sizeof_pos ge ty); lia. }
-  extlia.
-+ rewrite idlsize_app. 
-  erewrite tr_init_size by eauto. 
-  erewrite tr_init_array_size by eauto.
-  ring.
-
-- destruct 1; simpl; intros.
-+ rewrite padding_size by auto. lia.
-+ rewrite ! idlsize_app, padding_size. 
-  erewrite tr_init_size by eauto. 
-  rewrite <- (tr_init_struct_size _ _ _ _ _ H0 H1). lia.
-  unfold pos1. apply align_le. apply alignof_pos. 
-Qed.
+(* Hypothesis ce_consistent: composite_env_consistent ge. *)
 
 (** A semantics for general initializers *)
 
 Definition dummy_function := mkfunction Tvoid cc_default nil nil Sskip.
 
-Fixpoint fields_of_struct (fl: members) (pos: Z) : list (Z * type) :=
-  match fl with
-  | nil => nil
-  | (id1, ty1) :: fl' =>
-      (align pos (alignof ge ty1), ty1) :: fields_of_struct fl' (align pos (alignof ge ty1) + sizeof ge ty1)
+Fixpoint initialized_fields_of_struct (ms: members) (pos: Z) : res (list (Z * bitfield * type)) :=
+  match ms with
+  | nil =>
+      OK nil
+  | m :: ms' =>
+      let pos' := next_field ge.(genv_cenv) pos m in
+      if member_not_initialized m
+      then initialized_fields_of_struct ms' pos'
+      else
+        do ofs_bf <- layout_field ge.(genv_cenv) pos m;
+        do l <- initialized_fields_of_struct ms' pos';
+        OK ((ofs_bf, type_member m) :: l)
   end.
 
-Inductive exec_init: mem -> block -> Z -> type -> initializer -> mem -> Prop :=
-  | exec_init_single: forall m b ofs ty a v1 ty1 chunk m' v m'',
+Inductive exec_init: mem -> block -> Z -> bitfield -> type -> initializer -> mem -> Prop :=
+  | exec_init_single_: forall m b ofs bf ty a v1 ty1 m' v m'',
       star step ge (ExprState dummy_function a Kstop empty_env m)
                 E0 (ExprState dummy_function (Eval v1 ty1) Kstop empty_env m') ->
       sem_cast v1 ty1 ty m' = Some v ->
-      access_mode ty = By_value chunk ->
-      Mem.store chunk m' b ofs v = Some m'' ->
-      exec_init m b ofs ty (Init_single a) m''
+      exec_assign m' b ofs bf ty v m'' ->
+      exec_init m b ofs bf ty (Init_single a) m''
   | exec_init_array_: forall m b ofs ty sz a il m',
       exec_init_array m b ofs ty sz il m' ->
-      exec_init m b ofs (Tarray ty sz a) (Init_array il) m'
-  | exec_init_struct: forall m b ofs id a il co m',
+      exec_init m b ofs Full (Tarray ty sz a) (Init_array il) m'
+  | exec_init_struct_: forall m b ofs id a il co flds m',
       ge.(genv_cenv)!id = Some co -> co_su co = Struct ->
-      exec_init_list m b ofs (fields_of_struct (co_members co) 0) il m' ->
-      exec_init m b ofs (Tstruct id a) (Init_struct il) m'
-  | exec_init_union: forall m b ofs id a f i ty co m',
+      initialized_fields_of_struct (co_members co) 0 = OK flds ->
+      exec_init_struct m b ofs flds il m' ->
+      exec_init m b ofs Full (Tstruct id a) (Init_struct il) m'
+  | exec_init_union_: forall m b ofs id a f i co ty pos bf m',
       ge.(genv_cenv)!id = Some co -> co_su co = Union ->
       field_type f (co_members co) = OK ty ->
-      exec_init m b ofs ty i m' ->
-      exec_init m b ofs (Tunion id a) (Init_union f i) m'
+      union_field_offset ge f (co_members co) = OK (pos, bf) ->
+      exec_init m b (ofs + pos) bf ty i m' ->
+      exec_init m b ofs Full (Tunion id a) (Init_union f i) m'
 
 with exec_init_array: mem -> block -> Z -> type -> Z -> initializer_list -> mem -> Prop :=
   | exec_init_array_nil: forall m b ofs ty sz,
       sz >= 0 ->
       exec_init_array m b ofs ty sz Init_nil m
   | exec_init_array_cons: forall m b ofs ty sz i1 il m' m'',
-      exec_init m b ofs ty i1 m' ->
+      exec_init m b ofs Full ty i1 m' ->
       exec_init_array m' b (ofs + sizeof ge ty) ty (sz - 1) il m'' ->
       exec_init_array m b ofs ty sz (Init_cons i1 il) m''
 
-with exec_init_list: mem -> block -> Z -> list (Z * type) -> initializer_list -> mem -> Prop :=
-  | exec_init_list_nil: forall m b ofs,
-      exec_init_list m b ofs nil Init_nil m
-  | exec_init_list_cons: forall m b ofs pos ty l i1 il m' m'',
-      exec_init m b (ofs + pos) ty i1 m' ->
-      exec_init_list m' b ofs l il m'' ->
-      exec_init_list m b ofs ((pos, ty) :: l) (Init_cons i1 il) m''.
+with exec_init_struct: mem -> block -> Z -> list (Z * bitfield * type) -> initializer_list -> mem -> Prop :=
+  | exec_init_struct_nil: forall m b ofs,
+      exec_init_struct m b ofs nil Init_nil m
+  | exec_init_struct_cons: forall m b ofs pos bf ty l i1 il m' m'',
+      exec_init m b (ofs + pos) bf ty i1 m' ->
+      exec_init_struct m' b ofs l il m'' ->
+      exec_init_struct m b ofs ((pos, bf, ty) :: l) (Init_cons i1 il) m''.
 
 Scheme exec_init_ind3 := Minimality for exec_init Sort Prop
   with exec_init_array_ind3 := Minimality for exec_init_array Sort Prop
-  with exec_init_list_ind3 := Minimality for exec_init_list Sort Prop.
-Combined Scheme exec_init_scheme from exec_init_ind3, exec_init_array_ind3, exec_init_list_ind3.
+  with exec_init_struct_ind3 := Minimality for exec_init_struct Sort Prop.
+Combined Scheme exec_init_scheme from exec_init_ind3, exec_init_array_ind3, exec_init_struct_ind3.
 
 Remark exec_init_array_length:
   forall m b ofs ty sz il m',
@@ -809,87 +1256,95 @@ Proof.
   induction 1; lia.
 Qed.
 
-Lemma store_init_data_list_app:
-  forall data1 m b ofs m' data2 m'',
-  Genv.store_init_data_list ge m b ofs data1 = Some m' ->
-  Genv.store_init_data_list ge m' b (ofs + idlsize data1) data2 = Some m'' ->
-  Genv.store_init_data_list ge m b ofs (data1 ++ data2) = Some m''.
+Lemma transl_init_rec_sound:
+   (forall m b ofs bf ty i m',
+    exec_init m b ofs bf ty i m' ->
+    forall s s',
+    match_state s m b ->
+    match bf with
+    | Full => transl_init_rec ge s ty i ofs
+    | Bits sz sg p w => transl_init_bitfield ge s ty sz p w i ofs
+    end = OK s' ->
+    match_state s' m' b)
+/\ (forall m b ofs ty sz il m',
+    exec_init_array m b ofs ty sz il m' ->
+    forall s s',
+    match_state s m b ->
+    transl_init_array ge s ty il ofs = OK s' ->
+    match_state s' m' b)
+/\ (forall m b ofs flds il m',
+    exec_init_struct m b ofs flds il m' ->
+    forall s s' ms pos,
+    match_state s m b ->
+    initialized_fields_of_struct ms pos = OK flds ->
+    transl_init_struct ge s ms il ofs pos = OK s' ->
+    match_state s' m' b).
 Proof.
-  induction data1; simpl; intros.
-  inv H. rewrite Z.add_0_r in H0. auto.
-  destruct (Genv.store_init_data ge m b ofs a); try discriminate.
-  rewrite Z.add_assoc in H0. eauto.
-Qed.
-
-Remark store_init_data_list_padding:
-  forall frm to b ofs m,
-  Genv.store_init_data_list ge m b ofs (tr_padding frm to) = Some m.
-Proof.
-  intros. unfold tr_padding. destruct (zlt frm to); auto.
-Qed.
-
-Lemma tr_init_sound:
-  (forall m b ofs ty i m', exec_init m b ofs ty i m' ->
-   forall data, tr_init ty i data ->
-   Genv.store_init_data_list ge m b ofs data = Some m')
-/\(forall m b ofs ty sz il m', exec_init_array m b ofs ty sz il m' ->
-   forall data, tr_init_array ty il sz data ->
-   Genv.store_init_data_list ge m b ofs data = Some m')
-/\(forall m b ofs l il m', exec_init_list m b ofs l il m' ->
-   forall ty fl data pos,
-   l = fields_of_struct fl pos ->
-   tr_init_struct ty fl il pos data ->
-   Genv.store_init_data_list ge m b (ofs + pos) data = Some m').
-Proof.
-Local Opaque sizeof.
-  apply exec_init_scheme; simpl; intros.
+  apply exec_init_scheme.
 - (* single *)
-  inv H3. simpl. erewrite transl_init_single_steps by eauto. auto.
+  intros until m''; intros STEP CAST ASG s s' MS TR. destruct bf; monadInv TR.
+  + (* full *)
+    exploit transl_init_single_sound; eauto. intros [P Q].
+    eapply store_data_correct; eauto. 
+  + (* bitfield *)
+    destruct x; monadInv EQ0. monadInv EQ.
+    exploit constval_steps; eauto. intros [A [B C]]. subst m' ty1.
+    exploit sem_cast_match; eauto. intros D.
+    inv ASG. inv D.
+    set (f := first_bit sz pos width) in *.
+    assert (E: Vint c = Vint x) by (eapply load_int_correct; eauto).
+    inv E.
+    eapply store_int_correct; eauto.
 - (* array *)
-  inv H1. replace (Z.max 0 sz) with sz in H7. eauto.
-  assert (sz >= 0) by (eapply exec_init_array_length; eauto). extlia.
+  intros. monadInv H2. eauto.
 - (* struct *)
-  inv H3. unfold lookup_composite in H7. rewrite H in H7. inv H7. 
-  replace ofs with (ofs + 0) by lia. eauto.
+  intros. monadInv H5. unfold lookup_composite in EQ. rewrite H in EQ. inv EQ.
+  rewrite H0 in EQ0. eauto.
 - (* union *)
-  inv H4. unfold lookup_composite in H9. rewrite H in H9. inv H9. rewrite H1 in H12; inv H12. 
-  eapply store_init_data_list_app. eauto.
-  apply store_init_data_list_padding.
-
-- (* array, empty *)
-  inv H0; auto.
-- (* array, nonempty *)
-  inv H3.
-  eapply store_init_data_list_app.
+  intros. monadInv H6. unfold lookup_composite in EQ. rewrite H in EQ. inv EQ. rewrite H0 in EQ0.
+  rewrite H1, H2 in EQ0. simpl in EQ0. eauto.
+- (* array nil *)
+  intros. monadInv H1. auto.
+- (* array cons *)
+  intros. monadInv H4. eauto.
+- (* struct nil *)
+  intros. monadInv H1. auto.
+- (* struct cons *)
+  intros. simpl in H5. revert H4 H5. generalize pos0. induction ms as [ | m1 ms]. discriminate.
+  simpl. destruct (member_not_initialized m1).
+  intros; eapply IHms; eauto.
+  clear IHms. intros. monadInv H5. rewrite EQ in H4. monadInv H4. inv EQ0.
   eauto.
-  rewrite (tr_init_size _ _ _ H7). eauto.
-
-- (* struct, empty *)
-  inv H0. apply store_init_data_list_padding.
-- (* struct, nonempty *)
-  inv H4. simpl in H3; inv H3. 
-  eapply store_init_data_list_app. apply store_init_data_list_padding.
-  rewrite padding_size.
-  replace (ofs + pos0 + (pos2 - pos0)) with (ofs + pos2) by lia.
-  eapply store_init_data_list_app.
-  eauto.
-  rewrite (tr_init_size _ _ _ H9).
-  rewrite <- Z.add_assoc. eapply H2. eauto. eauto.
-  apply align_le. apply alignof_pos.
 Qed.
 
 End SOUNDNESS.
 
 Theorem transl_init_sound:
-  forall p m b ty i m' data,
-  exec_init (globalenv p) m b 0 ty i m' ->
+  forall p m b ty i m1 data,
+  let sz := sizeof (prog_comp_env p) ty in
+  Mem.range_perm m b 0 sz Cur Writable ->
+  reads_as_zeros m b 0 sz ->
+  exec_init (globalenv p) m b 0 Full ty i m1 ->
   transl_init (prog_comp_env p) ty i = OK data ->
-  Genv.store_init_data_list (globalenv p) m b 0 data = Some m'.
+  exists m2,
+     Genv.store_init_data_list (globalenv p) m b 0 data = Some m2
+  /\ Mem.loadbytes m2 b 0 (init_data_list_size data) = Mem.loadbytes m1 b 0 sz.
 Proof.
   intros.
   set (ge := globalenv p) in *.
-  change (prog_comp_env p) with (genv_cenv ge) in H0.
-  destruct (tr_init_sound ge) as (A & B & C).
-  eapply build_composite_env_consistent. apply prog_comp_env_eq.
-  eapply A; eauto. apply transl_init_spec; auto.
+  change (prog_comp_env p) with (genv_cenv ge) in *.
+  unfold transl_init in H2; monadInv H2.
+  fold sz in EQ. set (s0 := initial_state sz) in *.
+  assert (match_state ge s0 m b).
+  { constructor; simpl.
+  - generalize (sizeof_pos ge ty). fold sz. lia.
+  - apply Mem.loadbytes_empty. lia.
+  - auto.
+  - assumption.
+  }
+  assert (match_state ge x m1 b).
+  { eapply (proj1 (transl_init_rec_sound ge)); eauto. }
+  assert (total_size x = sz).
+  { change sz with s0.(total_size). eapply total_size_transl_init_rec; eauto. }
+  rewrite <- H4. eapply init_data_list_of_state_correct; eauto; rewrite H4; auto.
 Qed.
